Proved Theorem 2 of Santiago's POPL submission in our setting

UltimateSLH.v
@@ -555,3 +555,29 @@ Proof. (* from bcc + ideal_relative_secure *)
   apply ultimate_slh_bcc in Hev2; try assumption.
   eapply (ideal_relative_secure c st1 st2); eassumption.
 Qed.
+
+(* HIDE *)
+(* CH: Some playing with BCC generalization *)
+
+Definition ct_preservation trans : Prop := forall c,
+  (forall st1 st2 ast1 ast2, ideal_same_obs c st1 st2 ast1 ast2) ->
+  (forall st1 st2 ast1 ast2, spec_same_obs (trans c) st1 st2 ast1 ast2).
+
+(* Theorem 2 of Santiago's POPL submission *)
+Theorem ct_preservation_bw : forall trans,
+  (forall c, exists Td To, forall ds st ast ost st' ast' b,
+      <(st, ast, false, ds)> =[trans c]=> <(st', ast', b, ost)> ->
+     exists oss,
+      |-i <(st, ast, false, Td ds)> =[c]=> <(st', ast', b, oss)> /\
+      ost = To oss) ->
+  ct_preservation trans.
+Proof.
+  unfold ct_preservation, ideal_same_obs, spec_same_obs.
+  intros trans H c Hsrc st1 st2 ast1 ast2
+         ds stt1 stt2 astt1 astt2 bt1 bt2 os1 os2 H1 H2.
+  specialize (H c). destruct H as [Td [To H] ].
+  apply H in H1. destruct H1 as [oss1 [H1 H1'] ].
+  apply H in H2. destruct H2 as [oss2 [H2 H2'] ].
+  subst. f_equal. eapply Hsrc; eassumption.
+Qed.
+(* /HIDE *)
